\documentclass[12pt,a4paper]{article}
%
\setlength{\oddsidemargin}{  0mm}
\setlength{\topmargin}    { -12mm}
\setlength{\textheight}   { 246mm}
\setlength{\textwidth}    { 165mm}
\setlength{\parindent}    {  0   pt}  % not actually required but they

\setlength{\parskip}      {  6   pt}  % make paragraphs look less ugly

%

\usepackage{amsmath}
\usepackage{amssymb}
\usepackage{slashed}
\pagestyle{empty}

\include{Init}

\newcommand{\tphi}{\tilde{\phi}}
\newcommand{\tj}{\tilde{J}}
\newcommand{\tchi}{\tilde{\chi}}
\newcommand{\psibar}{\bar{\psi}}
\newcommand{\etabar}{\bar{\eta}}
\newcommand{\munu}{{\mu\nu}}

\begin{document}
\begin{center}
{\bf Quantum Field Theory}\\[\baselineskip]
\end{center}
{\bf Hogmanay's Problem Sheet}

\begin{enumerate}
\item {\it Change of scheme} \\

  Consider two renormalization schemes, leading to two definitions of
  the renormalized coupling, which we denote respectively $g(\mu)$ and
  $\tilde{g}(\mu)$. Clearly
  \[
    \tilde{g}(\mu) = F\left(g(\mu)\right)\, ,
  \]
  and we require
  \[
    F(x) = x + \frac{A}{3} x^3 + \ldots\, .
  \]
  The latter condition implies that the two couplings are the same at
  tree level and differ by quantum corrections, \ie the difference can
  be expanded in powers of $g^2$.

  Let us define (ignoring factors of 4 and $\pi$)
  \[
    \alpha(\mu) = g(\mu)^2\, , \quad \tilde{\alpha}(\mu) =
    \tilde{g}(\mu)^2\, .
  \]
  The $\beta$ function can be defined as the logarithmic derivative of
  $\alpha$ or $g$ -- and you will find both conventions in the
  literature:
  \[
    \mu\frac{d}{d\mu} \alpha(\mu) = \beta_\alpha(\alpha)\, , 
    \quad 
    \mu\frac{d}{d\mu} g(\mu) = \beta_g(g)\, . 
  \]
  Find the relation between $\beta_\alpha$ and $\beta_g$.

  If
  \[
    \beta_\alpha = C_1 \alpha^2 + C_2 \alpha^4 + \ldots\, ,
  \]
  and
  \[
    \tilde{\beta}_\alpha
    = \mu\frac{d}{d\mu} \tilde{\alpha}(\mu)
    = \tilde{C}_1 \tilde{\alpha}^2 + \tilde{C}_2 \tilde{\alpha}^4 +
    \ldots\, ,
  \]
  show that $C_1=\tilde{C}_1$ and $C_2=\tilde{C}_2$, i.e. the first
  two coefficients of the $\beta$ function are scheme-independent. 
  
  \bigskip
  
\item {\it $\Lambda$ parameter}\\

  Let us consider the following $\beta$ function:
  \[
    \mu\frac{d}{d\mu} g(\mu) = \beta(g) =-\beta_0 g^3 - \beta_1 g^5 +
    \ldots\, ,
  \]
  with $\beta_0,\beta_1>0$.
  Show that
  \[
    \lim_{\mu\to\infty} g(\mu) = 0\, ,
  \]
  integrate the RG equation at lowest order in perturbation theory,
  thereby showing that the running of the coupling is logarithmic.

  The RG equation can be rewritten as
  \[
    \frac{d\mu}{\mu} = \frac{dg}{\beta(g)}\, .
  \]
  Integrate this equation between two arbitrary scales, and then deduce that
  \[
    \Lambda = \mu \left(\beta_0 g(\mu)^2\right)^{-\beta_1/(2\beta_0^2))}\,
    e^{-1/(2\beta_0 g(\mu)^2)} \,
    \exp\left\{
      -\int_0^{g(\mu)} dx \left[
       \frac{1}{\beta(x)} + \frac{1}{\beta_0 x^3}-\frac{\beta_1}{\beta_0^2x} 
      \right]
    \right\}
  \]
  is independent of $\mu$. 

  \bigskip

\item {\it Scale dependence in $\phi^4$}\\

  Consider the $\phi^4$ theory in $D=4-2\epsilon$ dimensions,
  \[
    \mathcal{L} = \frac12 Z_\phi \partial_\mu \phi_R \partial^\mu \phi_R -
    \frac12 Z_m m_R^2 \phi_R^2 -\frac{1}{4!} Z_\lambda \lambda_R
    \phi_R^4\, .
  \]
  Compute the beta function to $O(\lambda^2)$, and the mass anomalous
  dimension to $O(\lambda)$.

  \bigskip
  
\item {\it Solution of RGEs for the two-point function}\\

  The Callan-Symanzik equation for the renormalized two-point function
  is
  \[
    \left[
      \mu \frac{\partial}{\partial \mu} + \beta(\bar\alpha)
      \frac{\partial}{\partial \bar\alpha} + \gamma_m(\bar\alpha)
      \bar{m} \frac{\partial}{\partial \bar{m}} +
      2 \gamma_\phi(\bar\alpha)
    \right] \Delta_{FR}(p^2; \bar\alpha, \bar{m}, \mu)=0\, , 
  \]
  where $\bar\alpha(\mu)$ and $\bar{m}(\mu)$ are renormalized
  couplings at the scale $\mu$.
 The product $\mu^2 \Delta_{FR}$ is dimensionless, and therefore
 invariant under rescaling of all dimensionful parameters, \viz
 \[
   \mu \mapsto e^\zeta \mu\, , \quad
   \bar{m} \mapsto e^\zeta \bar{m}\, , \quad
   p^\mu \mapsto e^\zeta p^\mu\, .
 \]
 Deduce that
 \[
   \left[
      \mu \frac{\partial}{\partial \mu} + 
      \bar{m} \frac{\partial}{\partial \bar{m}} +
      p \cdot \frac{\partial}{\partial p} - 2
    \right] \Delta_{FR}(p^2; \bar\alpha, \bar{m}, \mu)=0\, .
  \]
  Combining the two equations above, verify that
  \[
    \left[
      -p\cdot \frac{\partial}{\partial p} + \beta(\bar\alpha)
      \frac{\partial}{\partial \bar\alpha} - \left[1-
        \gamma_m(\bar\alpha)\right] 
      \bar{m} \frac{\partial}{\partial \bar{m}} +
      2 (1+\gamma_\phi(\bar\alpha))
    \right] \Delta_{FR}(p^2; \bar\alpha, \bar{m}, \mu)=0\, .
  \]
  Let $p^\mu=\lambda p'^\mu$, and show
  \[
    p\cdot \frac{\partial}{\partial p} \Delta_{FR}(p^2; \bar\alpha,
    \bar{m}, \mu) =
    \lambda \frac{\partial}{\partial\lambda} \Delta_{FR}((\lambda
    p')^2; \bar\alpha, \bar{m}, \mu)\, ,
  \]
  and therefore
  \[
    \left[
      -\lambda \frac{\partial}{\partial \lambda} + \beta(\bar\alpha)
      \frac{\partial}{\partial \bar\alpha} - \left[1-
        \gamma_m(\bar\alpha)\right] 
      \bar{m} \frac{\partial}{\partial \bar{m}} +
      2 (1+\gamma_\phi(\bar\alpha))
    \right] \Delta_{FR}((\lambda p)^2; \bar\alpha, \bar{m}, \mu)=0\, .
  \]
  In order to solve this equation, we set
  \[
    \lambda = e^{-t}\, , \quad \delta(\bar\alpha) = 2 +
    2\gamma_\phi(\bar\alpha)\, ,
  \]
  and hence:
  \[
    \left[
      \frac{\partial}{\partial t} + \beta(\bar\alpha)
      \frac{\partial}{\partial \bar\alpha} - \left[1-
        \gamma_m(\bar\alpha)\right] 
      \bar{m} \frac{\partial}{\partial \bar{m}} +
      \delta(\bar\alpha)
    \right] \Delta_{FR}((e^{-t} p)^2; \bar\alpha, \bar{m}, \mu)=0\, .
  \]
  Show that the running couplings
  \[
    \tilde\alpha(t) = \bar\alpha\left(e^t \mu\right)\, ,
    \quad
    \tilde{m}(t) = \bar{m}\left(e^t \mu\right)\, ,
  \]
  satisfy
  \[
    \frac{d}{dt} \tilde\alpha = \beta(\tilde\alpha) \, , \quad
    \frac{1}{\tilde{m}} \frac{d}{dt} \tilde{m} = -\left(
      1-\gamma_m(\tilde\alpha)
    \right)\, ,
  \]
  and finally that
  \[
    \left[\frac{d}{dt} + \delta(\tilde\alpha) \right]
    \Delta_{FR}((e^{-t} p)^2; \tilde\alpha, \tilde{m}, \mu)=0\, . 
  \]
  Solve this equation and show that
  \[
    \Delta_{FR}\left((e^t p)^2; \bar\alpha, \bar{m}, \mu\right) =
    \Delta_{FR}(p^2; \tilde\alpha(t), \tilde{m}(t), \mu)
    \exp\left[\int_0^t dt' \delta\left(\tilde\alpha(t')\right)\right]
    \, .
  \]
  Show that in the absence of divergences, \ie for
  \[
    \beta=\gamma_m=\gamma_\phi=0\, ,
  \]
  the equation above reproduces the naive scaling predicted from
  dimensional analysis. This should clarify why $\gamma_m$ and
  $\gamma_\phi$ are called anomalous dimensions.

  Note that this analysis can be extended to any correlator of fields,
  with straightforward modifications. 
\end{enumerate}

\vfill
\hspace*{\fill}\tiny L Del Debbio, December 2018.
\end{document}
